fsharp/Realized/Zen.Array.Base.fs
@@ -1,0 +1,37 @@
+#light "off"
+module Zen.Array.Base
+
+open Microsoft.FSharp.Core.Operators.Checked // For checked casts
+
+module Arr = Microsoft.FSharp.Collections.Array
+module Cost = Zen.Cost.Realized
+
+type t<'A> = array<'A>
+type indexed<'A, 'Dummy> = array<'A>
+
+let length (arr: array<'A>): Prims.nat =
+    Arr.length arr
+    |> int64
+
+let get ( _: Prims.nat)
+        ( arr : indexed<'Aa, Prims.unit> )
+        ( i : Prims.nat)
+        : 'Aa =
+    arr.[int i]
+
+let empty (): indexed<'Aa, Prims.unit> = [||]
+
+let empty_uniq (): unit = ()
+
+let ofList (ls: Prims.list<'A>): Cost.t<indexed<'A, Prims.unit>, Prims.unit> =
+    let rec toList acc = function
+        | Prims.Nil -> acc
+        | Prims.Cons(hd, tl) -> toList (hd::acc) tl
+    in
+    lazy(
+        ls |> toList[]
+           |> List.rev
+           |> Array.ofList
+    ) |> Cost.C
+
+let ofList_get (_: Prims.list<'A>) (_:Prims.nat): unit = () 
