fstar/Zen.ContractResult.fst
@@ -3,29 +3,32 @@ module Zen.ContractResult
 open Zen.Base
 open Zen.Types
 open Zen.Cost
-
-module R = Zen.Result
+module RT = Zen.ResultT
 module CReturn = Zen.ContractReturn
+
 type t = contractResult
 
-let ofTxSkel: txSkeleton -> contractResult =
-    CReturn.ofTxSkel >> OK
+let ofTxSkel: txSkeleton -> contractResult `cost` 3 =
+    CReturn.ofTxSkel >> RT.liftCost
 
-let ofResultTxSkel: result txSkeleton -> contractResult =
-    R.map CReturn.ofTxSkel
+let ofResultTxSkel(tx: result txSkeleton): contractResult `cost` 3 =
+    let open RT in
+    RT.liftRes tx >>= ofTxSkel
 
-val ofOptionTxSkel: string -> option txSkeleton -> contractResult
-let ofOptionTxSkel msg =
-    R.ofOption "msg"
-    >> ofResultTxSkel
+val ofOptionTxSkel: string -> option txSkeleton -> contractResult `cost` 3
+let ofOptionTxSkel msg tx =
+    RT.ofOption "msg" tx
+    >>= ofResultTxSkel
 
-let setMessage: message -> contractResult -> contractResult =
-    R.map << CReturn.setMessage
-let setState: stateUpdate -> contractResult -> contractResult =
-    R.map << CReturn.setState
-let setStateDelete: contractResult -> contractResult =
+let setMessage (msg: message) (cRes: contractResult): contractResult `cost` 3 =
+    let open RT in
+    RT.liftRes cRes >>= (CReturn.setMessage msg >> RT.liftCost)
+let setState (update: stateUpdate) (cRes: contractResult): contractResult `cost` 3 =
+    let open RT in
+    RT.liftRes cRes >>= (CReturn.setState update >> RT.liftCost)
+let setStateDelete: contractResult -> contractResult `cost` 3 =
     setState Delete
-let setStateNoChange: contractResult -> contractResult =
+let setStateNoChange: contractResult -> contractResult `cost` 3 =
     setState NoChange
-let setStateUpdate: data -> contractResult -> contractResult =
+let setStateUpdate: data -> contractResult -> contractResult `cost` 3 =
     setState << Update
