fstar/Zen.ContractReturn.fst
@@ -2,24 +2,25 @@ module Zen.ContractReturn
 
 open Zen.Base
 open Zen.Types
+open Zen.Cost
 
 type t = contractReturn
 
-val ofTxSkel: txSkeleton -> contractReturn
-let ofTxSkel txSkel = {tx=txSkel; message=None; state=NoChange}
+val ofTxSkel: txSkeleton -> contractReturn `cost` 3
+let ofTxSkel txSkel = {tx=txSkel; message=None; state=NoChange} |> incRet 3
 
-val setTx: txSkeleton -> contractReturn -> contractReturn
-let setTx txSkel contractReturn = {contractReturn with tx=txSkel}
+val setTx: txSkeleton -> contractReturn -> contractReturn `cost` 3
+let setTx txSkel cReturn = {cReturn with tx=txSkel} |> incRet 3
 
-val setMessage: message -> contractReturn -> contractReturn
-let setMessage msg contractReturn = {contractReturn with message=Some msg}
+val setMessage: message -> contractReturn -> contractReturn `cost` 3
+let setMessage msg cReturn = {cReturn with message=Some msg} |> incRet 3
 
-val setState: stateUpdate -> contractReturn -> contractReturn
-let setState sUpdate contractReturn = {contractReturn with state=sUpdate}
+val setState: stateUpdate -> contractReturn -> contractReturn `cost` 3
+let setState sUpdate cReturn = {cReturn with state=sUpdate} |> incRet 3
 
-let setStateDelete: contractReturn -> contractReturn =
+let setStateDelete: contractReturn -> contractReturn `cost` 3 =
     setState Delete
-let setStateNoChange: contractReturn -> contractReturn =
+let setStateNoChange: contractReturn -> contractReturn `cost` 3 =
     setState NoChange
-let setStateUpdate: data -> contractReturn -> contractReturn =
+let setStateUpdate: data -> contractReturn -> contractReturn `cost` 3 =
     setState << Update
