fstar/Zen.Array.Base.fsti
@@ -1,0 +1,32 @@
+module Zen.Array.Base
+
+open Zen.Cost
+
+type t (a:Type) = array a
+
+(** Gets the length of the array *)
+val length(#a:Type): array a -> nat
+
+type indexed (a:Type) (l:nat) = arr:array a{length arr == l}
+
+(** accesses an array at i *)
+val get(#a:Type)(#l:nat): arr:indexed a l -> i:nat{i < l} -> a
+
+(** The empty array *)
+val empty: indexed 'a 0
+
+(** The empty array is the unique array with length 0 *)
+val empty_uniq: unit -> Lemma (forall (a:Type) (arr: array a).
+                               length arr == 0 <==> arr == empty)
+
+(** Converts a list to an array *)
+val ofList(#a:Type):
+    ls:list a
+    -> indexed a (Prims.length ls) `cost` (Prims.length ls * 2 + 2)
+
+(** The element of `Array.ofList ls` at `i` is equal to `List.nth ls i` *)
+val ofList_get(#a:Type):
+    ls:list a
+    -> i:nat{i < Prims.length ls}
+    -> Lemma (let arr = ofList ls in
+              get (force arr) i == force (Zen.List.nth ls i))
