fstar/Zen.Array.Indexed.fst
@@ -1,0 +1,127 @@
+module Zen.Array.Indexed
+
+open Zen.Base
+open Zen.Cost
+open Zen.Array.Base
+
+type t (a: Type) (n: nat) = indexed a n
+
+val ofArray(#a:Type): array a -> l:nat & indexed a l
+let ofArray #_ arr = (|length arr, arr|)
+
+val toList(#a:Type)(#l:nat):
+    indexed a l
+    -> ls:list a{Prims.length ls == l} `cost` (l * 2 + 2)
+let toList #a #l arr =
+    let rec buildList: i:nat{i<=l} -> ls:list a{Prims.length ls == i} = function
+        | 0 -> []
+        | i -> get arr (l-i) :: buildList (i-1)
+    in
+    buildList l |> incRet (l * 2 + 2)
+
+unfold val item(#a:Type)(#l:nat): i:nat{i < l} -> arr:indexed a l -> a
+unfold let item #_ #_ i arr = get arr i
+
+unfold val op_Array_Access(#a:Type)(#l:nat): arr:indexed a l -> i:nat{i < l} -> a
+unfold let op_Array_Access #_ #_ arr i = get arr i
+
+val init_pure(#a:Type)(#n:nat):
+    l:nat
+    -> f:(i:nat{i<l} -> a `cost` n)
+    -> indexed a l `cost` (l * (n+4) + 4)
+let init_pure #a #_ l f =
+    Zen.List.init_pure_length l f;
+    Zen.List.init_pure l f `bind_dep` (fun (ls:list a{Prims.length ls == l}) ->
+        Zen.Array.Base.ofList ls <: indexed a l `cost` (l * 2 + 2))
+
+val init(#a:Type)(#n:nat):
+    l:nat
+    -> f:(nat -> a `cost` n)
+    -> indexed a l `cost` (l * (n+4) + 4)
+let init #_ #_ l f = init_pure l f
+
+(** create returns an array of length l in which each element is x. *)
+val create(#a:Type): l:nat -> x:a -> indexed a l `cost` (l * 4 + 4)
+let create(#_) l x = init l (konst x >> ret)
+
+(** sub returns the subrange of arr from i to (i+j). *)
+val sub(#a:Type)(#l:nat): arr:indexed a l -> i:nat{i<l} -> j:nat{i+j <= l}
+  -> cost (indexed a j) (j * 4 + 4)
+let sub #a #l arr i j =
+    let rec buildList: k:nat{k <= j} -> ls:list a{Prims.length ls == k} =
+        function
+        | 0 -> []
+        | k -> get arr (i+j-k) :: buildList (k-1)
+    in
+    (ofList (buildList j) <: indexed a j `cost` (j * 2 + 2))
+    |> inc (j * 2 + 2)
+
+(** Creates an array whose elements are the results of applying the supplied function to each of the elements of a supplied array. *)
+val map(#a #b:Type)(#n #l:nat): (a -> cost b n) -> indexed a l
+  -> cost (indexed b l) (l * (n+4) + 4)
+let map #a #_ #_ #l f arr = init_pure l (get arr >> f)
+
+
+(** `append a1 a2` returns an array containing the elements of a1 followed by the elements of a2. *)
+val append(#a:Type)(#l1 #l2:nat): indexed a l1 -> indexed a l2
+  -> cost (indexed a (l1+l2)) ((l1+l2) * 4 + 4)
+let append #a #l1 #l2 a1 a2 =
+  let fetch (i:nat{ i < (l1+l2)}): a =
+    if i < l1 then a1.(i) else a2.(i-l1)
+  in
+  if l1 + l2 = 0 then empty |> incRet 4 else
+  init_pure (l1+l2) (fetch >> ret)
+
+
+(*
+(** [concat3 a1 a2 a3] returns an array containing the elements of a1 followed by the elements of a2 followed by the elements of a3. *)
+val concat3(#a:Type)(#l1 #l2 #l3:nat): indexed a l1 -> indexed a l2 -> indexed a l3
+  -> cost (indexed a (l1+l2+l3)) (2 * (l1+l2+l3))
+let concat3 #_ #l1 #l2 #l3 a1 a2 a3 =
+  let fetch (i:nat{ i < (l1+l2+l3)}) = if i < l1      then a1.(i)
+                                  else if i < l1 + l2 then a2.(i-l1)
+                                  else                     a3.(i-l1-l2)
+  in
+  if (l1+l2+l3) = 0 then ret empty else
+  init (l1+l2+l3) fetch
+*)
+val chunkBySize(#a:Type)(#l:nat):
+    size:pos
+    -> a `indexed` l
+    -> indexed (indexed a size) (l / size)
+       `cost`
+       ((l/size)*(4*size+8) + 4)
+let chunkBySize #a #l size arr =
+    let chunk (i: nat{i < (l / size)})
+              : indexed a size `cost` (4*size+4) =
+              assert(i <= (l/size) - 1);
+              sub arr (i * size) size
+    in
+    if l / size = 0 then empty |> incRet 4 else
+    init_pure (l / size) chunk
+
+val joinOptions(#a:Type)(#l:nat):
+    indexed (option a) l
+    -> option (indexed a l) `cost` (l * 4 + 4)
+let joinOptions #a #l arr =
+    let rec buildList
+        (i:nat{i <= l})
+        : option (ls:list a{Prims.length ls == i}) =
+        match i with
+        | 0 -> Some []
+        | i -> begin match get arr (l-i), buildList (i-1) with
+               | Some x, Some xs -> Some (x::xs)
+               | _ -> None
+               end
+    in
+    match buildList l with
+    | Some xs -> (ofList xs <: (indexed a l `cost` (l * 2 + 2)))
+                 >>= Zen.OptionT.incSome (l * 2 + 2)
+    | None -> Zen.OptionT.incNone (l * 4 + 4)
+
+val tryMap(#a #b:Type)(#l #n:nat):
+    (a -> option b `cost` n)
+    -> indexed a l
+    -> option (indexed b l) `cost` (l * (n + 8) + 8)
+let tryMap #_ #_ #_ #_ f arr =
+    map f arr >>= joinOptions
