fstar/Zen.Array.fst
@@ -1,3 +1,3 @@
 module Zen.Array
-include Zen.Array.Realized
-include Zen.Array.Extracted
+include Zen.Array.Indexed
+include Zen.Array.Base
