fstar/Zen.Hash.Base.fst
@@ -1,0 +1,9 @@
+module Zen.Hash.Base
+
+open Zen.Cost
+open Zen.Types
+
+type t = hash
+
+unfold val parse: string -> option hash `cost` 32
+unfold let parse = Zen.Crypto.parseHash
