fstar/Zen.Hash.fst
@@ -1,0 +1,3 @@
+module Zen.Hash
+include Zen.Hash.Sha3
+include Zen.Hash.Base
