tests/Zen.Array.fsx
@@ -7,41 +7,41 @@ open FsCheck
 
 module C = Zen.Cost.Realized
 module P = Prims
-module ZAR = Zen.Array.Realized
-module ZAE = Zen.Array.Extracted
+module ZAB = Zen.Array.Base
+module ZAI = Zen.Array.Indexed
 
 type ArrayProperties =
 
     static member ``zLength equivalent to fsLength`` (zs: int[]) =
-        ZAR.length zs = int64 (zs.Length)
+        ZAB.length zs = int64 (zs.Length)
 
     static member ``zItem equivalent to fsItem`` (i: int) (zs: int[]) =
         (0 < i && i < zs.Length) ==>
-        lazy ( let zItem = ZAR.item (ZAR.length zs) (int64 i) zs
+        lazy ( let zItem = ZAI.item (ZAB.length zs) (int64 i) zs
                let fsItem = zs.[i]
-               C.__force zItem = fsItem )
+               zItem = fsItem )
 
     static member ``zInit equivalent to fsInit`` (zs: int[]) =
-        let n = ZAR.length zs
+        let n = ZAB.length zs
         (n <> 0L && n < int64 System.Int32.MaxValue) ==>
-        lazy ( let zInit = ZAR.init 0L n (fun i -> ZAR.item (ZAR.length zs) i zs)
+        lazy ( let zInit = ZAI.init 0L n (fun i -> ZAI.item (ZAB.length zs) i zs |> C.ret)
                let fsInit = Array.init (int n) (fun i -> zs.[i])
                C.__force zInit = fsInit )
 
     static member ``zGet equivalent to fsItem`` (i: int) (zs: int[]) =
         (0 < i && i < zs.Length) ==>
-        lazy ( let zGet = ZAE.get (ZAR.length zs) zs (int64 i)
+        lazy ( let zGet = ZAB.get (ZAB.length zs) zs (int64 i)
                let fsItem = zs.[i]
-               C.__force zGet = fsItem )
+               zGet = fsItem )
 
     static member ``zAt equivalent to fsItem`` (i: int) (zs: int[]) =
         (0 < i && i < zs.Length) ==>
-        lazy ( let zAt = ZAE.get (ZAR.length zs) zs (int64 i)
+        lazy ( let zAt = ZAB.get (ZAB.length zs) zs (int64 i)
                let fsItem = zs.[i]
-               C.__force zAt = fsItem )
+               zAt = fsItem )
 
     static member ``zCreate equivalent to fsCreate`` (n: int) (x: int) =
-        0 < n ==> lazy ( let zCreate = ZAE.create (int64 n) x
+        0 < n ==> lazy ( let zCreate = ZAI.create (int64 n) x
                          let fsCreate = Array.create n x
                          C.__force zCreate = fsCreate )
 
@@ -53,7 +53,7 @@ type ArrayProperties =
         let j = int j
         let n = zs.Length
         i + j <= n ==>
-        lazy ( let zSub = ZAE.sub (int64 n) zs (int64 i) (int64 j)
+        lazy ( let zSub = ZAI.sub (int64 n) zs (int64 i) (int64 j)
                let fsSub = Array.sub zs i j
                C.__force zSub = fsSub )
 
@@ -61,12 +61,12 @@ type ArrayProperties =
         (zs: int[])
         (f: Function<int, byte>) =
         let f = f.Value
-        let zMap = ZAE.map 0L (ZAR.length zs) (f >> C.ret) zs
+        let zMap = ZAI.map 0L (ZAB.length zs) (f >> C.ret) zs
         let fsMap = Array.map f zs
         C.__force zMap = fsMap
 
     static member ``zAppend equivalent to fsAppend`` (xs: int[]) (ys: int[]) =
-        let zAppend = ZAE.append (ZAR.length xs) (ZAR.length ys) xs ys
+        let zAppend = ZAI.append (ZAB.length xs) (ZAB.length ys) xs ys
         let fsAppend = Array.append xs ys
         C.__force zAppend = fsAppend
 
@@ -74,7 +74,7 @@ type ArrayProperties =
         (sz: PositiveInt)
         (zs: int[]) =
         let sz = int sz
-        let zChunks = ZAE.chunkBySize (ZAR.length zs) (int64 sz) zs
+        let zChunks = ZAI.chunkBySize (ZAB.length zs) (int64 sz) zs
         let fsChunks = Array.chunkBySize sz zs
         (C.__force zChunks).Length = zs.Length / sz
         &&
