verify.sh
@@ -1,7 +1,7 @@
 #!/bin/sh
 
-mono ../../packages/ZFStar/tools/fstar.exe \
-     --smt ../../packages/zen_z3_linux/output/z3-linux \
+mono packages/ZFStar/tools/fstar.exe \
+     --smt packages/zen_z3_linux/output/z3-linux \
      --prims fstar/prims.fst \
      --no_default_includes \
      --include $PWD/fstar \
